Prove Equiv_ctx2 (formerly Equiv_ctx_weak)

linking/context_equiv.v
@@ -86,14 +86,14 @@ Definition Equiv_ctx (ge : ge_ty) (N : pos) plt (p1 p2 : Prog.t N) :=
       (terminates (link_ctx C p1 plt) ge c1 m1 
    <-> terminates (link_ctx C p2 plt) ge c2 m2).
 
-(** A weaker notion of contextual equivalence, in which the initial memory [m]
+(** An alternate of contextual equivalence, in which the initial memory [m]
  is equal in source and target (this is possible, e.g., if [m] contains just
  globals). [m] must self-inject. 
 
- The advantage of the weaker notion is that it is easily shown to be a preorder
- (reflexive and transitive). *)
+ The advantage of this alternate notion is that it is easily shown reflexive and
+ transitive. *)
 
-Definition Equiv_ctx_weak (ge : ge_ty) (N : pos) plt (p1 p2 : Prog.t N) :=
+Definition Equiv_ctx2 (ge : ge_ty) (N : pos) plt (p1 p2 : Prog.t N) :=
   forall C : Ctx.t ge,
   forall (main : val) (args : list val) m,
   cc_init_inv (Mem.flat_inj (Mem.nextblock m)) ge args m ge args m -> 
@@ -105,13 +105,13 @@ Definition Equiv_ctx_weak (ge : ge_ty) (N : pos) plt (p1 p2 : Prog.t N) :=
     & (terminates (link_ctx C p1 plt) ge c1 m 
    <-> terminates (link_ctx C p2 plt) ge c2 m)].
 
-Lemma Equiv_ctx_weak_refl ge N plt (p : Prog.t N) : Equiv_ctx_weak ge plt p p.
+Lemma Equiv_ctx2_refl ge N plt (p : Prog.t N) : Equiv_ctx2 ge plt p p.
 Proof. by move=> C main args m Inv c1 -> Hsafe; exists c1; split. Qed.
 
-Lemma Equiv_ctx_weak_trans ge N plt (p1 p2 p3 : Prog.t N) : 
-  Equiv_ctx_weak ge plt p1 p2 -> 
-  Equiv_ctx_weak ge plt p2 p3 -> 
-  Equiv_ctx_weak ge plt p1 p3.
+Lemma Equiv_ctx2_trans ge N plt (p1 p2 p3 : Prog.t N) : 
+  Equiv_ctx2 ge plt p1 p2 -> 
+  Equiv_ctx2 ge plt p2 p3 -> 
+  Equiv_ctx2 ge plt p1 p3.
 Proof. 
 move=> H1 H2 C main args m Inv c1 Init1 Hsafe.
 case (H1 C main args m Inv c1 Init1 Hsafe)=> c2 []Init2 Hsafe2 Hterm12.
@@ -173,6 +173,61 @@ Qed.
 End ContextEquiv.
 
 End ContextEquiv.
+
+(** Prove that Simulation implies Equiv_ctx2 *)
+
+Module ContextEquiv2 (LS : LINKING_SIMULATION). 
+                                                                       
+Import LS.                                                             
+                                                                       
+Section ContextEquiv.
+
+Variable N : pos.
+Variable pS pT : Prog.t N.
+Variable rclosed_S : forall ix : 'I_N, RCSem.t (Prog.sems pS ix).(sem) (Prog.sems pS ix).(ge).
+Variable valid_T : forall ix : 'I_N, Nuke_sem.t (Prog.sems pT ix).(sem).
+Variable targets_det : forall ix : 'I_N, corestep_fun (Prog.sems pT ix).(sem).
+Variable plt : ident -> option 'I_N.
+Variable sims : 
+  forall ix : 'I_N,                                          
+  let s := Prog.sems pS ix in                                              
+  let t := Prog.sems pT ix in                                              
+  SM_simulation_inject s.(sem) t.(sem) s.(ge) t.(ge).
+Variable ge_top : ge_ty.                                                     
+Variable domeq_S : forall ix : 'I_N, genvs_domain_eq ge_top (Prog.sems pS ix).(ge).
+Variable domeq_T : forall ix : 'I_N, genvs_domain_eq ge_top (Prog.sems pT ix).(ge). 
+Variable find_symbol_ST : 
+  forall (ix : 'I_N) id bf, 
+  Genv.find_symbol (ge (Prog.sems pS ix)) id = Some bf -> 
+  Genv.find_symbol (ge (Prog.sems pT ix)) id = Some bf.
+
+Lemma equiv : Equiv_ctx2 ge_top plt pS pT.
+Proof.
+rewrite /Equiv_ctx=> C main args m Init c1 Init1 Hsafe.
+have sim: CompCert_wholeprog_sim (link_ctx C pS plt) (link_ctx C pT plt) ge_top ge_top main.
+{ apply: link=> ix; rewrite /Prog.sems/apply_ctx/extend_sems. 
+  by move=> ??; case e: (lt_dec ix N)=> [pf|pf] //; apply find_symbol_ST.
+  by case e: (lt_dec ix N)=> [pf|pf] //; apply: (Ctx.rclosed_C C).
+  by case e: (lt_dec ix N)=> [pf|pf] //; apply: (Ctx.valid_C C).
+  by case e: (lt_dec ix N)=> [pf|pf] //; apply: (Ctx.sim_C C).
+  by case e: (lt_dec ix N)=> [pf|pf] //; apply: (Ctx.domeq_C C).
+  by case e: (lt_dec ix N)=> [pf|pf] //; apply: (Ctx.domeq_C C). }
+have target_det: corestep_fun (link_ctx C pT plt). 
+{ apply: linking_det=> ix; rewrite /Prog.sems/apply_ctx/extend_sems.
+  by case e: (lt_dec ix N)=> [pf|pf] //; apply Ctx.det_C. }
+eapply @core_initial 
+  with (Sem1 := link_ctx C pS plt) (Sem2 := link_ctx C pT plt) 
+       (ge1 := ge_top) (ge2 := ge_top) (halt_inv := cc_halt_inv)
+       (j := Mem.flat_inj (Mem.nextblock m)) (main := main) (m1 := m) (m2 := m) (w := sim)
+  in Init1; eauto.
+case: Init1=> mu []cd []c2 []_ []Init2' Hmatch.
+exists c2; split=> //; first by eapply safety_preservation; eauto.
+by apply equitermination in Hmatch.
+Qed.
+
+End ContextEquiv.
+
+End ContextEquiv2.
 
 
 
